euclidean uniqueness for divmod does not hold on word

src/MachineWidth32.v
@@ -7,6 +7,33 @@ Import Word.ArithmeticNotations.
 Local Open Scope word_scope.
 Local Open Scope Z_scope.
 
+Lemma NToWord_plus: forall sz (n m : N), NToWord sz (n + m) = NToWord sz n ^+ NToWord sz m.
+Admitted.
+
+Lemma NToWord_inj: forall sz (n m: N),
+    NToWord sz n = NToWord sz m ->
+    (n < Npow2 sz)%N ->
+    (m < Npow2 sz)%N ->
+    n = m.
+Admitted.
+
+Ltac Nify_one n :=
+    rewrite <- (NToWord_wordToN n) in *;
+    let B := fresh "B" in
+    pose proof (wordToN_bound n) as B;
+    rewrite (wordToN_NToWord_2 _ B) in *;
+    let E := fresh "E" in
+    let n' := fresh n in
+    remember (wordToN n) as n' eqn: E;
+    clear E n;
+    rename n' into n.
+
+Ltac Nify :=
+  repeat match goal with
+  | n: word _ |- _ => Nify_one n
+  end.
+
+Definition TODO{T: Type}: T. Admitted.
 
 Instance MachineWidth32: MachineWidth (word 32) := {|
   add := @wplus 32;
@@ -64,6 +91,61 @@ Instance MachineWidth32: MachineWidth (word 32) := {|
   ZToReg_regToZ_signed := @ZToWord_wordToZ 32;
   XLEN_lbound := ltac:(lia);
 |}.
+all: intros.
+- split.
+  + unfold wdiv, wmod, wmult, wordBin.
+    rewrite wordToN_NToWord_2 by apply TODO.
+    rewrite <- NToWord_plus.
+    rewrite <- (N.div_mod' (wordToN a) (wordToN b)).
+    rewrite NToWord_wordToN.
+    reflexivity.
+  + split.
+    * pose proof uwordToZ_bound as P.
+      (* automation_challenge *)
+      specialize (P 32%nat (a ^% b)). intuition idtac.
+    * unfold uwordToZ.
+      apply N2Z.inj_lt.
+      unfold wmod, wordBin.
+      assert (wordToN a mod wordToN b < wordToN b)%N. {
+        apply N.mod_upper_bound. rewrite ZToWord_0 in H. apply wordToN_neq_0. assumption.
+      }
+      rewrite wordToN_NToWord_2; [assumption|].
+      eapply N.lt_trans; [eassumption|].
+      apply wordToN_bound.
+- unfold wdiv, wmod, wmult, wordBin, uwordToZ in *.
+  Nify.
+  destruct H0 as [E [_ R]].
+  apply N2Z.inj_lt in R.
+  rewrite <- NToWord_plus in E.
+  apply NToWord_inj in E.
+  + split; f_equal.
+    * apply N.div_unique in E; assumption.
+    * apply N.mod_unique in E; assumption.
+  + assumption.
+  + apply TODO. (* does not hold!
+
+  uniqueness of div does not hold on word:
+  Example with sz = 4 (i.e. everything is modulo 16).
+
+  Given a=13, b=8, there are several ways to satisfy the equation
+  a  = b * q + r    0 <= r < b
+  13 = 8 * 1 + 5    0 <= 5 < 8
+  13 = 8 * 3 + 5    0 <= 5 < 8
+  13 = 8 * 5 + 5    0 <= 5 < 8
+  etc
+
+  uniqueness of mod does not hold either:
+
+  Given a=13, b=14, there are several ways to satisfy the equation
+  a  =  b * q +  r    0 <=  r <  b
+  13 = 14 * 0 + 13    0 <= 13 < 14
+  13 = 14 * 3 +  3    0 <=  3 < 14
+  
+  a = b * q + r    0 <= r < b
+  
+  3 = 8 * 8 + 3    0 <= 3 < 8
+ *)
+Defined.
 
 Goal False.
   idtac "Testing that all operations reduce under cbv."
